Refactor Coq examples

Coq/src/Example.v
@@ -12,6 +12,8 @@ Set Implicit Arguments.
 
 Definition coin := Coin__Bool.
 Definition share := Share.
+Definition T : Prog bool := pure true.
+Definition F : Prog bool := pure false.
 Definition const := fun A (x _ : A) => x.
 
 Section exB.
@@ -24,7 +26,7 @@ Section exB.
   Example example3 : Prog bool :=  share coin >>= fun fx => fx ? fx.
   Example res_example3 := [true; false; true; false].
   
-  Example exOr0 : Prog bool := orM coin (pure false).
+  Example exOr0 : Prog bool := orM coin F.
   Example res_exOr0 := [true; false].
   
   Example exOr1 : Prog bool := orM coin coin.
@@ -34,14 +36,14 @@ Section exB.
   Example res_exOr2 := [true; false].
   
   Example exOr2a : Prog bool :=
-    share coin >>= fun fx => orM (pure false) (orM fx fx).
+    share coin >>= fun fx => orM F (orM fx fx).
   Example res_exOr2a := [true; false].
   
   Example exOr2b : Prog bool :=
-    share coin >>= fun fx => orM (pure true) (orM fx fx).
+    share coin >>= fun fx => orM T (orM fx fx).
   Example res_exOr2b := [true].
   
-  Example exOr3 : Prog bool := orM (coin ? coin) (pure true).
+  Example exOr3 : Prog bool := orM (coin ? coin) T.
   Example res_exOr3 := [true; true; true; true].
   
   Example exOr3a : Prog bool := orM (coin ? coin) coin.
@@ -66,10 +68,10 @@ Section exB.
   Example exOr7 : Prog bool := share coin >>= fun fx => orM coin (orM fx fx).
   Example res_exOr7 := [true; true; false].
   
-  Example exOr7a : Prog bool := share coin >>= fun fx => orM (pure true) (orM fx fx).
+  Example exOr7a : Prog bool := share coin >>= fun fx => orM T (orM fx fx).
   Example res_exOr7a := [true].
   
-  Example exOr7b : Prog bool := share coin >>= fun fx => orM (pure false) (orM fx fx).
+  Example exOr7b : Prog bool := share coin >>= fun fx => orM F (orM fx fx).
   Example res_exOr7b := [true; false].
   
   Example exShareConst : Prog bool := share coin >>= fun fx => const fx fx.
@@ -81,71 +83,76 @@ Section exB.
   Example exShareConstOrL : Prog bool := share coin >>= fun fx => orM (const fx fx) fx.
   Example res_exShareConstOrL := [true; false].
   
-  Example exShareConstOrR2 : Prog bool := share coin >>= fun fx => orM (pure true) (const fx fx).
+  Example exShareConstOrR2 : Prog bool := share coin >>= fun fx => orM T (const fx fx).
   Example res_exShareConstOrR2 := [true].
   
-  Example exFailed : Prog bool := share Fail >>= fun fx => const (pure true) fx.
+  Example exFailed : Prog bool := share Fail >>= fun fx => const T fx.
   Example res_exFailed := [true].
   
   Example exHead : Prog bool := headM (consM coin Fail).
   Example res_exHead := [true; false].
   
   Example exOrShareShare : Prog bool :=
-    share coin >>=
-          fun fx =>
-            share coin >>=
-                  fun fy =>
-                    orM fx (orM fy (orM fx fy)).
+    share coin >>= fun fx =>
+    share coin >>= fun fy =>
+      orM fx (orM fy (orM fx fy)).
   Example res_exOrShareShare := [true; true; false].
   
   Example exOrShareNested : Prog bool :=
     share coin >>= fun fx =>
-                     orM fx (share coin >>= fun fy =>
-                                              orM fy (orM fx fy)).
+    orM fx (share coin >>= fun fy =>
+      orM fy (orM fx fy)).
   Example res_exOrShareNested := [true; true; false].
   
   Example exShareNestedChoiceOr : Prog bool :=
-    share ((pure true ? pure false) ? (pure true ? pure false)) >>=
-          fun fx => orM fx fx.
+    share ((pure true ? pure false) ? (pure true ? pure false)) >>= fun fx =>
+      orM fx fx.
   Example res_exShareNestedChoiceOr := [true; false; true; false].
   
   Example exShareIgnoreShare : Prog bool :=
-    share coin >>= fun fx => const (pure true) (share fx >>= fun fy => orM fy fy).
+    share coin >>= fun fx =>
+      const T (share fx >>= fun fy => orM fy fy).
   Example res_exShareIgnoreShare := [true].
   
   Example exRepeatedShare : Prog bool :=
     share coin >>= fun fx => share fx >>= fun fy => orM fy fy.
   Example res_exRepeatedShare := [true; false].
+
+ Example exSkipIds : Prog bool :=
+    Share coin >>= fun fx => const coin (const fx fx).
+  Example res_exSkipIds := [true; false].
   
-  Definition exBs := [(example1, res_example1);
-                        (example2, res_example2);
-                        (example3, res_example3);
-                        (exOr0, res_exOr0);
-                        (exOr1, res_exOr1);
-                        (exOr2, res_exOr2);
-                        (exOr2a, res_exOr2a);
-                        (exOr2b, res_exOr2b);
-                        (exOr3, res_exOr3);
-                        (exOr3a, res_exOr3a);
-                        (exOr3b, res_exOr3b);
-                        (exOr3c, res_exOr3c);
-                        (exOr4, res_exOr4);
-                        (exOrShare, res_exOrShare);
-                        (exOr6, res_exOr6);
-                        (exOr7, res_exOr7);
-                        (exOr7a, res_exOr7a);
-                        (exOr7b, res_exOr7b);
-                        (exShareConst, res_exShareConst);
-                        (exShareConstOrR, res_exShareConstOrR);
-                        (exShareConstOrL, res_exShareConstOrL);
-                        (exShareConstOrR2, res_exShareConstOrR2);
-                        (exFailed, res_exFailed);
-                        (exHead, res_exHead);
-                        (exOrShareShare, res_exOrShareShare);
-                        (exOrShareNested, res_exOrShareNested);
-                        (exShareNestedChoiceOr, res_exShareNestedChoiceOr);
-                        (exShareIgnoreShare, res_exShareIgnoreShare);
-                        (exRepeatedShare, res_exRepeatedShare)].
+  Definition exBs :=
+    [(example1, res_example1);
+       (example2, res_example2);
+       (example3, res_example3);
+       (exOr0, res_exOr0);
+       (exOr1, res_exOr1);
+       (exOr2, res_exOr2);
+       (exOr2a, res_exOr2a);
+       (exOr2b, res_exOr2b);
+       (exOr3, res_exOr3);
+       (exOr3a, res_exOr3a);
+       (exOr3b, res_exOr3b);
+       (exOr3c, res_exOr3c);
+       (exOr4, res_exOr4);
+       (exOrShare, res_exOrShare);
+       (exOr6, res_exOr6);
+       (exOr7, res_exOr7);
+       (exOr7a, res_exOr7a);
+       (exOr7b, res_exOr7b);
+       (exShareConst, res_exShareConst);
+       (exShareConstOrR, res_exShareConstOrR);
+       (exShareConstOrL, res_exShareConstOrL);
+       (exShareConstOrR2, res_exShareConstOrR2);
+       (exFailed, res_exFailed);
+       (exHead, res_exHead);
+       (exOrShareShare, res_exOrShareShare);
+       (exOrShareNested, res_exOrShareNested);
+       (exShareNestedChoiceOr, res_exShareNestedChoiceOr);
+       (exShareIgnoreShare, res_exShareIgnoreShare);
+       (exRepeatedShare, res_exRepeatedShare);
+       (exSkipIds, res_exSkipIds)].
   
   Lemma tests__exBs : Forall (fun '(p,r) => handle p = r) exBs.
   Proof. repeat econstructor. Qed.
@@ -153,49 +160,55 @@ End exB.
 
 Section exPB.
   Example exDup : Prog (Pair bool bool) := dup coin.
-  Example res_exDup := [Pair' (pure true) (pure true)
-                        ; Pair' (pure true) (pure false)
-                        ; Pair' (pure false) (pure true)
-                        ; Pair' (pure false) (pure false)].
+  Example res_exDup := [Pair' T T
+                        ; Pair' T F
+                        ; Pair' F T
+                        ; Pair' F F].
   
   Example exDupShare : Prog (Pair bool bool) := share coin >>= fun x => dup x.
-  Example res_exDupShare := [Pair' (pure true) (pure true)
-                             ; Pair' (pure false) (pure false)].
+  Example res_exDupShare := [Pair' T T; Pair' F F].
   
   Example exDupShare2 : Prog (Pair bool bool) := dupShare coin.
 
-  Example res_exDupShare2 := [Pair' (pure true) (pure true)
-                              ; Pair' (pure false) (pure false)].
+  Example res_exDupShare2 := [Pair' T T; Pair' F F].
   
-  Example exDupFailed : Prog (Pair bool bool) := share Fail >>= fun x => dup (const (pure true) x).
-  Example res_exDupFailed := [Pair' (pure true) (pure true)].
+  Example exDupFailed : Prog (Pair bool bool) := share Fail >>= fun x => dup (const T x).
+  Example res_exDupFailed := [Pair' T T].
   
   Example exDupFirst : Prog (Pair bool bool) := dup (firstM (pairM coin (@Fail bool))).
-  Example res_exDupFirst := [Pair' (pure true) (pure true)
-                             ; Pair' (pure true) (pure false)
-                             ; Pair' (pure false) (pure true)
-                             ; Pair' (pure false) (pure false)].
+  Example res_exDupFirst := [Pair' T T
+                             ; Pair' T F
+                             ; Pair' F T
+                             ; Pair' F F].
   
   Example exDupShareFirst : Prog (Pair bool bool) := dupShare (@firstM bool bool (pairM coin Fail)).
-  Example res_exDupShareFirst :=  [Pair' (pure true) (pure true); Pair' (pure false) (pure false)].
+  Example res_exDupShareFirst :=  [Pair' T T; Pair' F F].
 
   
   Example exShareNestedChoice : Prog (Pair bool bool) :=
-    share ((pure true ? pure false) ? (pure true ? pure false)) >>=
-          fun fx => pairM fx fx.
-  Example res_exShareNestedChoice := [Pair' (pure true) (pure true) 
-                                      ; Pair' (pure false) (pure false)
-                                      ; Pair' (pure true) (pure true)
-                                      ; Pair' (pure false) (pure false)].
+    share ((pure true ? pure false) ? (pure true ? pure false)) >>= fun fx =>
+      pairM fx fx.
+  Example res_exShareNestedChoice := [Pair' T T 
+                                      ; Pair' F F
+                                      ; Pair' T T
+                                      ; Pair' F F].
   
-  Definition exPBs := [(exDup, res_exDup)
-                       ; (exDupShare, res_exDupShare)
-                       ; (exDupShare2, res_exDupShare2)
-                       ; (exDupFailed, res_exDupFailed)
-                       ; (exDupFirst, res_exDupFirst)
-                       ; (exDupShareFirst, res_exDupShareFirst)
-                       ; (exShareNestedChoice, res_exShareNestedChoice)].
+ 
+  Example exShareInShare : Prog (Pair bool bool) :=
+    Share (Share coin >>= fun fx => orM fx fx) >>= fun fy => pairM fy fy.
+  Example res_exShareInShare := [Pair' T T
+                                 ; Pair' F F].
 
+  Definition exPBs :=
+    [(exDup, res_exDup)
+     ; (exDupShare, res_exDupShare)
+     ; (exDupShare2, res_exDupShare2)
+     ; (exDupFailed, res_exDupFailed)
+     ; (exDupFirst, res_exDupFirst)
+     ; (exDupShareFirst, res_exDupShareFirst)
+     ; (exShareNestedChoice, res_exShareNestedChoice)
+     ; (exShareInShare, res_exShareInShare)].
+  
   Lemma tests__exPBs : Forall (fun '(p,r) => handle p = r) exPBs.
   Proof. repeat econstructor. Qed.
 End exPB.
@@ -205,145 +218,128 @@ Section exLB.
   Arguments Nil' {_}.
 
   Example exDupl : Prog (List bool) := dupl (headM (consM coin Fail)).
-  Example res_exDupl := [Cons' (pure true) (consM (pure true) nilM)
-                         ; Cons' (pure true) (consM (pure false) nilM)
-                         ; Cons' (pure false) (consM (pure true) nilM)
-                         ; Cons' (pure false) (consM (pure false) nilM)].
+  Example res_exDupl := [Cons' T (consM T nilM)
+                         ; Cons' T (consM F nilM)
+                         ; Cons' F (consM T nilM)
+                         ; Cons' F (consM F nilM)].
 
   Example exDupl2 : Prog (List bool) := consM (headM (consM coin Fail))
                                            (consM (headM (consM coin Fail)) nilM).
-  Example res_exDupl2 := [Cons' (pure true) (consM (pure true) nilM)
-                          ; Cons' (pure true) (consM (pure false) nilM)
-                          ; Cons' (pure false) (consM (pure true) nilM)
-                          ; Cons' (pure false) (consM (pure false) nilM)].
+  Example res_exDupl2 := [Cons' T (consM T nilM)
+                          ; Cons' T (consM F nilM)
+                          ; Cons' F (consM T nilM)
+                          ; Cons' F (consM F nilM)].
 
   Example exDuplShare : Prog (List bool) := duplShare (headM (consM coin Fail)).
-  Example res_exDuplShare := [Cons' (pure true) (consM (pure true) nilM)
-                              ; Cons' (pure false) (consM (pure false) nilM)].
+  Example res_exDuplShare := [Cons' T (consM T nilM)
+                              ; Cons' F (consM F nilM)].
 
   Example exShareNestedChoice2 : Prog (List bool) :=
-    share (pure true ? (pure false ? pure true)) >>=
-          fun fx => share coin >>= fun fy => consM fx (consM fy (consM fx (consM fy nilM))).
+    share (pure true ? (pure false ? pure true)) >>= fun fx =>
+    share coin >>= fun fy =>
+      consM fx (consM fy (consM fx (consM fy nilM))).
 
   Example res_exShareNestedChoice2 :=
-    [Cons' (pure true) (consM (pure true) (consM (pure true) (consM (pure true) nilM)))
-     ; Cons' (pure true) (consM (pure false) (consM (pure true) (consM (pure false) nilM)))
-     ; Cons' (pure false) (consM (pure true) (consM (pure false) (consM (pure true) nilM)))
-     ; Cons' (pure false) (consM (pure false) (consM (pure false) (consM (pure false) nilM)))
-     ; Cons' (pure true) (consM (pure true) (consM (pure true) (consM (pure true) nilM)))
-     ; Cons' (pure true) (consM (pure false) (consM (pure true) (consM (pure false) nilM)))].
+    [Cons' T (consM T (consM T (consM T nilM)))
+     ; Cons' T (consM F (consM T (consM F nilM)))
+     ; Cons' F (consM T (consM F (consM T nilM)))
+     ; Cons' F (consM F (consM F (consM F nilM)))
+     ; Cons' T (consM T (consM T (consM T nilM)))
+     ; Cons' T (consM F (consM T (consM F nilM)))].
 
   Example exOrShareNestedList : Prog (List bool) :=
     share coin >>= fun fx =>
-                     consM fx (share coin >>= fun fy =>
-                                                consM fy (consM fx (consM fy nilM))).
+    consM fx (share coin >>= fun fy =>
+      consM fy (consM fx (consM fy nilM))).
+
   Example res_exOrShareNestedList :=
-    [Cons' (pure true) (consM (pure true) (consM (pure true) (consM (pure true) nilM)))
-     ; Cons' (pure true) (consM (pure false) (consM (pure true) (consM (pure false) nilM)))
-     ; Cons' (pure false) (consM (pure true) (consM (pure false) (consM (pure true) nilM)))
-     ; Cons' (pure false) (consM (pure false) (consM (pure false) (consM (pure false) nilM)))].
+    [Cons' T (consM T (consM T (consM T nilM)))
+     ; Cons' T (consM F (consM T (consM F nilM)))
+     ; Cons' F (consM T (consM F (consM T nilM)))
+     ; Cons' F (consM F (consM F (consM F nilM)))].
 
-  Definition exLBs := [(exDupl, res_exDupl)
-                       ; (exDupl2,  res_exDupl2)
-                       ; (exDuplShare, res_exDuplShare)
-                       ; (exShareNestedChoice2, res_exShareNestedChoice2)
-                       ; (exOrShareNestedList, res_exOrShareNestedList)].
-
-  Lemma tests__exLBs : Forall (fun '(p,r) => handle p = r) exLBs.
-  Proof. repeat econstructor. Qed.
-
-End exLB.
-              
-Section exLPB.
-
- Example exShareSingleton : Prog (Pair (List bool) (List bool)) :=
-   Share (consM (pure true ? pure false) nilM) >>= fun fx => pairM fx fx.
- Example res_exShareSingleton := [Pair' (pure (Cons' (pure true) nilM))
-                                        (pure (Cons' (pure true) nilM))
-                                  ; Pair' (pure (Cons' (pure false) nilM))
-                                          (pure (Cons' (pure false) nilM))].
-
-   Fixpoint recList' (n : nat) (xs : List bool) : Prog (List bool) :=
-     match n with
-     | 0 => Fail
-     | S n => match xs with
-             | Nil' _ => nilM
-             | Cons' fy fys =>
-               Share fys >>= fun fys' => consM (notM fy) (fys' ? fys' >>= fun zs => recList' n zs)
-             end
-     end.
-
-   
-   Definition recList (fxs : Prog (List bool)) : Prog (List bool) :=
-     fxs >>= fun xfps => lengthM xfps >>= fun fuel => recList' (fuel + 1) xfps.
-
-   Example exRecList : Prog (Pair (List bool) (List bool)) :=
-     Share (recList (consM (pure true) (consM (pure false) nilM))) >>= fun fx => pairM fx fx.
-   Example res_exRecList :=  [ Pair' (consM (pure false) (consM (pure false) nilM))
-                                     (consM (pure false) (consM (pure false) nilM))
-                             ; Pair' (consM (pure false) (consM (pure true) nilM))
-                                     (consM (pure false) (consM (pure true) nilM))
-                             ; Pair' (consM (pure false) (consM (pure true) nilM))
-                                     (consM (pure false) (consM (pure true) nilM))].
-   
-   Definition exLPBs := [(exShareSingleton, res_exShareSingleton)
-                         ; (exRecList, res_exRecList)].
-   
-  Lemma tests__exLPBs : Forall (fun '(p,r) => handle p = r) exLPBs.
-  Proof. repeat econstructor. Qed.
-End exLPB.
-
-Section Extra.
-  Example exSkipIds : Prog bool :=
-    Share coin >>= fun fx => const coin (const fx fx).
-  Example res_exSkipIds := [true; false].
-
-  Lemma lem_exSkipIDs : handle exSkipIds = res_exSkipIds.
-  Proof. reflexivity. Qed.
-
-  Example exShareInShare : Prog (Pair bool bool) :=
-    Share (Share coin >>= fun fx => orM fx fx) >>= fun fy => pairM fy fy.
-  Example res_exShareInShare := [Pair' (pure true) (pure true)
-                                 ; Pair' (pure false) (pure false)].
-  Lemma lem_exShareInShare : handle exShareInShare = res_exShareInShare.
-  Proof. reflexivity. Qed.
-
-  Example exShareListInShare : Prog (Pair (List bool) (List bool)) :=
-    Share (Share (consM coin (consM coin nilM)) >>=
-                 fun fx => appM fx fx) >>= fun fy => pairM fy fy.
+  Fixpoint recList' (xs : List bool) : Prog (List bool) :=
+    match xs with
+    | Nil' => nilM
+    | Cons' fy fys => consM (notM fy)
+                           (fys ? fys >>= fun zs => recList' zs)
+    end.
   
-  Example res_exShareListInShare :=
-    [Pair' (consM (pure true) (consM (pure true) (consM (pure true) (consM (pure true) nilM))))
-           (consM (pure true) (consM (pure true) (consM (pure true) (consM (pure true) nilM))))
-     ; Pair' (consM (pure true) (consM (pure false) (consM (pure true) (consM (pure false) nilM))))
-             (consM (pure true) (consM (pure false) (consM (pure true) (consM (pure false) nilM))))
-     ; Pair' (consM (pure false) (consM (pure true) (consM (pure false) (consM (pure true) nilM))))
-             (consM (pure false) (consM (pure true) (consM (pure false) (consM (pure true) nilM))))
-     ; Pair' (consM (pure false) (consM (pure false) (consM (pure false) (consM (pure false) nilM))))
-             (consM (pure false) (consM (pure false) (consM (pure false) (consM (pure false) nilM))))].
-  Lemma lem_exShareListInShare : handle exShareListInShare = res_exShareListInShare.
-  Proof. reflexivity. Qed.
+  Definition recList (fxs : Prog (List bool)) : Prog (List bool) :=
+    fxs >>= fun xs => recList' xs.
+  
+  Example exRecList : Prog (List bool) :=
+    recList (consM T (consM F nilM)).
+  Example res_exRecList :=  [(Cons' F (consM F nilM))
+                             ; (Cons' F (consM T nilM))
+                             ; (Cons' F (consM T nilM))].
 
   Example exSharePutPos : Prog (List bool) :=
     Share (Share (consM coin nilM) >>= fun fx => appM fx fx) >>= fun fy => appM fy fy.
   
-  Example res_exSharePutPos := [Cons' (pure true) (consM (pure true) (consM (pure true) (consM (pure true) nilM)))
-                                ; Cons'  (pure false) (consM (pure false) (consM (pure false) (consM (pure false) nilM)))].
-  Lemma lem_exSharePutPos : handle exSharePutPos = res_exSharePutPos.
-  Proof. reflexivity. Qed.
+  Example res_exSharePutPos := [Cons' T (consM T (consM T (consM T nilM)))
+                                ; Cons'  F (consM F (consM F (consM F nilM)))].
 
   Example exShareListInRepeatedShare : Prog (List bool) :=
     Share (Share (consM coin nilM) >>= fun fx => appM fx fx) >>=
           fun fy => Share coin >>= fun fz => Share coin >>= fun fa => consM fz (consM fa fy).
   Example res_exShareListInRepeatedShare :=
-    [Cons' (pure true) (consM (pure true) (consM (pure true) (consM (pure true) nilM)))
-     ; Cons' (pure true) (consM (pure true) (consM (pure false) (consM (pure false) nilM)))
-     ;  Cons' (pure true) (consM (pure false) (consM (pure true) (consM (pure true) nilM)))
-     ;  Cons' (pure true) (consM (pure false) (consM (pure false) (consM (pure false) nilM)))
-     ;  Cons' (pure false) (consM (pure true) (consM (pure true) (consM (pure true) nilM)))
-     ;  Cons' (pure false) (consM (pure true) (consM (pure false) (consM (pure false) nilM)))
-     ;  Cons' (pure false) (consM (pure false) (consM (pure true) (consM (pure true) nilM)))
-     ;  Cons' (pure false) (consM (pure false) (consM (pure false) (consM (pure false) nilM)))].
-  Lemma lem_exShareListInRepeatedShare : handle exShareListInRepeatedShare = res_exShareListInRepeatedShare.
-  Proof. reflexivity. Qed.
-End Extra.
+    [Cons' T (consM T (consM T (consM T nilM)))
+     ; Cons' T (consM T (consM F (consM F nilM)))
+     ;  Cons' T (consM F (consM T (consM T nilM)))
+     ;  Cons' T (consM F (consM F (consM F nilM)))
+     ;  Cons' F (consM T (consM T (consM T nilM)))
+     ;  Cons' F (consM T (consM F (consM F nilM)))
+     ;  Cons' F (consM F (consM T (consM T nilM)))
+     ;  Cons' F (consM F (consM F (consM F nilM)))].
+
+  Definition exLBs :=
+    [(exDupl, res_exDupl)
+     ; (exDupl2,  res_exDupl2)
+     ; (exDuplShare, res_exDuplShare)
+     ; (exShareNestedChoice2, res_exShareNestedChoice2)
+     ; (exOrShareNestedList, res_exOrShareNestedList)
+     ; (exRecList, res_exRecList)
+     ; (exSharePutPos, res_exSharePutPos)
+     ; (exShareListInRepeatedShare, res_exShareListInRepeatedShare)].
+
+  Lemma tests__exLBs : Forall (fun '(p,r) => handle p = r) exLBs.
+  Proof. repeat econstructor. Qed.
+End exLB.
+              
+Section exLPB.
+ Example exShareSingleton : Prog (Pair (List bool) (List bool)) :=
+   Share (consM (pure true ? pure false) nilM) >>= fun fx =>
+     pairM fx fx.
+ Example res_exShareSingleton := [Pair' (pure (Cons' T nilM))
+                                        (pure (Cons' T nilM))
+                                  ; Pair' (pure (Cons' F nilM))
+                                          (pure (Cons' F nilM))].
+
+ 
+ Definition exLPBs := [(exShareSingleton, res_exShareSingleton)].
+ 
+ Lemma tests__exLPBs : Forall (fun '(p,r) => handle p = r) exLPBs.
+ Proof. repeat econstructor. Qed.
+End exLPB.
+
+Section exPLB.
+  Example exShareListInShare : Prog (Pair (List bool) (List bool)) :=
+    Share (Share (consM coin (consM coin nilM)) >>=
+                 fun fx => appM fx fx) >>= fun fy => pairM fy fy.
+  
+  Example res_exShareListInShare :=
+    [Pair' (consM T (consM T (consM T (consM T nilM))))
+           (consM T (consM T (consM T (consM T nilM))))
+     ; Pair' (consM T (consM F (consM T (consM F nilM))))
+             (consM T (consM F (consM T (consM F nilM))))
+     ; Pair' (consM F (consM T (consM F (consM T nilM))))
+             (consM F (consM T (consM F (consM T nilM))))
+     ; Pair' (consM F (consM F (consM F (consM F nilM))))
+             (consM F (consM F (consM F (consM F nilM))))].
+
+  Definition exPLBs := [(exShareListInShare, res_exShareListInShare)].
+ 
+ Lemma tests__exPLBs : Forall (fun '(p,r) => handle p = r) exPLBs.
+ Proof. repeat econstructor. Qed.
+End exPLB.
